cflow/src/timer_event_internal.h
@@ -18,4 +18,3 @@ cflow_timer_event_fire_result cflow_timer_event_queue_commit_claim(
     cflow_timer_event_claim *claim);
 
 #endif /* CFLOW_TIMER_EVENT_INTERNAL_H */
-
